nondeterministic_dataflow/table_1/B8.thy
@@ -9,11 +9,11 @@ no_notation Sublist.parallel (infixl "\<parallel>" 50)
 section \<open>Axiom B8\<close>
 lemma B8_gen:
   \<open> (transp_op (case_sum buf A) :: ('a :: {countable,defaults} + 0, 0 + 'a, 'b) op) ~ map_op id (case_sum Inr Inl) (id_op (case_sum buf A))\<close>
-proof (coinduction arbitrary: buf rule: bisim_coinduct_upto'')
+proof (coinduction arbitrary: buf rule: bisim_coinduct)
   case SIM1
   then show ?case 
   proof -
-    have "\<exists>op2'. step (Inp p x) (map_op id (case_sum Inr Inl) (id_op (case_sum buf A))) op2' \<and> bisim_cong (\<lambda>op1xx op2xx. \<exists>buf. op1xx = transp_op (case_sum buf A) \<and> op2xx = map_op id (case_sum Inr Inl) (id_op (case_sum buf A))) (transp_op (BENQ p x (case_sum buf A))) op2'"
+    have "\<exists>op2'. step (Inp p x) (map_op id (case_sum Inr Inl) (id_op (case_sum buf A))) op2' \<and> bisim_R (\<lambda>op1xx op2xx. \<exists>buf. op1xx = transp_op (case_sum buf A) \<and> op2xx = map_op id (case_sum Inr Inl) (id_op (case_sum buf A))) (transp_op (BENQ p x (case_sum buf A))) op2'"
       if "p \<notin> defaults"
       for p :: "'a + 0"
         and x :: 'b
@@ -21,7 +21,7 @@ proof (coinduction arbitrary: buf rule: bisim_coinduct_upto'')
     proof (cases p)
       case (Inl a)
       from this that show ?thesis 
-       apply (intro exI conjI[rotated,OF bc_base])
+       apply (intro exI conjI[rotated,OF b_base])
        apply (intro conjI)
       apply simp
       apply (rule refl)+
@@ -32,12 +32,12 @@ proof (coinduction arbitrary: buf rule: bisim_coinduct_upto'')
       from this that show ?thesis 
         by force
     qed
-    moreover have "\<exists>op2'. step (Out (Inr x2) (BHD x2 buf)) (map_op id (case_sum Inr Inl) (id_op (case_sum buf A))) op2' \<and> bisim_cong (\<lambda>op1xx op2xx. \<exists>buf. op1xx = transp_op (case_sum buf A) \<and> op2xx = map_op id (case_sum Inr Inl) (id_op (case_sum buf A))) (transp_op (case_sum (BTL x2 buf) A)) op2'"
+    moreover have "\<exists>op2'. step (Out (Inr x2) (BHD x2 buf)) (map_op id (case_sum Inr Inl) (id_op (case_sum buf A))) op2' \<and> bisim_R (\<lambda>op1xx op2xx. \<exists>buf. op1xx = transp_op (case_sum buf A) \<and> op2xx = map_op id (case_sum Inr Inl) (id_op (case_sum buf A))) (transp_op (case_sum (BTL x2 buf) A)) op2'"
       if "x2 \<notin> defaults"
         and "buf x2 \<noteq> []"
       for x2 :: 'a
       using that 
-       apply (intro exI conjI[rotated,OF bc_base])
+       apply (intro exI conjI[rotated,OF b_base])
        apply (intro conjI)
       apply simp
       apply (rule refl)+
@@ -50,7 +50,7 @@ next
   case SIM2
   then show ?case 
   proof -
-    have "\<exists>op2'. step (Inp p x) (transp_op (case_sum buf A)) op2' \<and> bisim_cong (\<lambda>op1xx op2xx. \<exists>buf. op1xx = transp_op (case_sum buf A) \<and> op2xx = map_op id (case_sum Inr Inl) (id_op (case_sum buf A))) op2' (map_op id (case_sum Inr Inl) (id_op (BENQ p x (case_sum buf A))))"
+    have "\<exists>op2'. step (Inp p x) (transp_op (case_sum buf A)) op2' \<and> bisim_R (\<lambda>op1xx op2xx. \<exists>buf. op1xx = transp_op (case_sum buf A) \<and> op2xx = map_op id (case_sum Inr Inl) (id_op (case_sum buf A))) op2' (map_op id (case_sum Inr Inl) (id_op (BENQ p x (case_sum buf A))))"
       if "p \<notin> defaults"
       for p :: "'a + 0"
         and x :: 'b
@@ -58,7 +58,7 @@ next
     proof (cases p)
       case (Inl a)
       from this that show ?thesis 
-       apply (intro exI conjI[rotated,OF bc_base])
+       apply (intro exI conjI[rotated,OF b_base])
        apply (intro conjI)
           apply simp
         apply simp
@@ -69,12 +69,12 @@ next
       from this that show ?thesis 
         by force
     qed
-    moreover have "\<exists>op2'. step (Out (Inr x1) (BHD x1 buf)) (transp_op (case_sum buf A)) op2' \<and> bisim_cong (\<lambda>op1xx op2xx. \<exists>buf. op1xx = transp_op (case_sum buf A) \<and> op2xx = map_op id (case_sum Inr Inl) (id_op (case_sum buf A))) op2' (map_op id (case_sum Inr Inl) (id_op (case_sum (BTL x1 buf) A)))"
+    moreover have "\<exists>op2'. step (Out (Inr x1) (BHD x1 buf)) (transp_op (case_sum buf A)) op2' \<and> bisim_R (\<lambda>op1xx op2xx. \<exists>buf. op1xx = transp_op (case_sum buf A) \<and> op2xx = map_op id (case_sum Inr Inl) (id_op (case_sum buf A))) op2' (map_op id (case_sum Inr Inl) (id_op (case_sum (BTL x1 buf) A)))"
       if "x1 \<notin> defaults"
         and "buf x1 \<noteq> []"
       for x1 :: 'a
       using that 
-       apply (intro exI conjI[rotated,OF bc_base])
+       apply (intro exI conjI[rotated,OF b_base])
        apply (intro conjI)
       apply simp
       apply (rule refl)+
